Define AsmC

x86/AsmC.v
@@ -1,11 +1,10 @@
-Require Import Coqlib Maps.
-Require Import AST Integers Floats Values Memory Events Globalenvs Smallstep.
+Require Import CoqlibC Maps.
+Require Import ASTC Integers Floats Values MemoryC Events Globalenvs Smallstep.
 Require Import Locations Stacklayout Conventions.
 (** newly added **)
-Require Import Asmregs.
 Require Export Asm.
-Require Import ModSem.
-Require Import CoqlibC.
+Require Import Simulation AsmregsC.
+Require Import Skeleton ModSem Mod.
 
 Set Implicit Arguments.
 
@@ -34,78 +33,265 @@ Definition st_m (st0: state): mem :=
   end
 .
 
+Section ASMEXTRA.
+
+  Definition is_external (ge: genv) (st: state): Prop :=
+    match Genv.find_funct ge (st.(st_rs) PC) with
+    | Some (AST.External ef) => is_external_ef ef
+    | _ => False
+    end
+  .
+
+  Variable ge: genv.
+  Definition semantics_with_ge := Semantics step bot1 final_state ge.
+  (* *************** ge is parameterized *******************)
+
+  Lemma semantics_receptive
+        st
+        (INTERNAL: ~is_external semantics_with_ge.(globalenv) st)
+    :
+      receptive_at semantics_with_ge st
+  .
+  Proof.
+    admit "this should hold".
+  Qed.
+
+  Lemma semantics_determinate
+        st
+        (INTERNAL: ~is_external semantics_with_ge.(globalenv) st)
+    :
+      determinate_at semantics_with_ge st
+  .
+  Proof.
+    admit "this should hold".
+  Qed.
+
+End ASMEXTRA.
+(*** !!!!!!!!!!!!!!! REMOVE ABOVE AFTER MERGING WITH MIXED SIM BRANCH !!!!!!!!!!!!!!!!!! ***)
+
+
+
+
+
+
+
+
+
+
+
+
+
+
+
+
+
+
+
+
 Section MODSEM.
 
+  Variable skenv_link: SkEnv.t.
   Variable p: program.
-  Let ge := p.(Genv.globalenv).
+  Let skenv: SkEnv.t := skenv_link.(SkEnv.project) p.(defs).
+  Let ge: genv := skenv.(SkEnv.revive) p.
 
+  Record state := mkstate {
+    init_rs: regset;
+    st: Asm.state;
+  }.
 
-  (* Inductive at_external: state -> val -> option signature -> regset -> mem -> Prop := *)
-  (* | at_external_intro *)
-  (*     rs_arg m_arg b_arg *)
-  (*     (FPTR: rs_arg # PC = Vptr b_arg Ptrofs.zero true) *)
-  (*     (EXTERNAL: Genv.find_funct_ptr ge b_arg = None) *)
-  (*   : *)
-  (*     at_external (State rs_arg m_arg) (Vptr b_arg Ptrofs.zero true) None rs_arg m_arg *)
-  (* . *)
-
-  Inductive at_external (st0: state): regset -> mem -> Prop :=
+  Inductive at_external (skenv_link: SkEnv.t): state -> Args.t -> Prop :=
   | at_external_intro
-      fb_arg
-      (FPTR: st0.(st_rs) # PC = Vptr fb_arg Ptrofs.zero true)
-      (EXTERNAL: Genv.find_funct_ptr ge fb_arg = None)
-      fd
-      (RAINTERNAL: Genv.find_funct ge (st0.(st_rs) # RA) = Some (Internal fd)) (* Only for disjointness with final_frame *)
+      rs m0 m1 fptr sg vs blk ofs
+      (FPTR: rs # PC = fptr)
+      (EXTERNAL: Genv.find_funct ge fptr = None)
+      (SIG: exists skd, skenv_link.(Genv.find_funct) fptr = Some skd /\ SkEnv.get_sig skd = sg)
+      (VALS: extcall_arguments rs m0 sg vs)
+      (RSP: rs RSP = Vptr blk ofs true)
+      (FREE: Mem.free m0 blk ofs.(Ptrofs.unsigned) (1 + ofs.(Ptrofs.unsigned) + (size_arguments sg)) = Some m1)
+      init_rs
     :
-      at_external st0 st0.(st_rs) st0.(st_m)
+      at_external skenv_link (mkstate init_rs (State rs m0)) (Args.mk fptr vs m0)
   .
 
-  Inductive initial_frame (rs_arg: regset) (m_arg: mem)
+  Inductive initial_frame (args: Args.t)
     : state -> Prop :=
   | initial_frame_intro
+      fd m0 rs blk
+      (FINDF: Genv.find_funct ge args.(Args.fptr) = Some (Internal fd))
+      (ALLOC: Mem.alloc args.(Args.m) 0 (size_arguments fd.(fn_sig)) = (m0, blk))
+      (PC: rs # PC = args.(Args.fptr))
+      (RPS: rs # RSP = Vptr blk Ptrofs.zero true)
+      (VALS: extcall_arguments rs m0 fd.(fn_sig) args.(Args.vs))
     :
-      initial_frame rs_arg m_arg (State rs_arg m_arg)
+      initial_frame args (mkstate rs (State rs m0))
   .
 
-  Inductive final_frame (rs_init: regset) (st0: state): regset -> Prop :=
+  Inductive final_frame: state -> Retv.t -> Prop :=
   | final_frame_intro
-      fb
-      (FPTR: st0.(st_rs) # PC = Vptr fb Ptrofs.zero true)
-      (EXTERNAL: Genv.find_funct_ptr ge fb = None)
-      (RA: st0.(st_rs) # PC = st0.(st_rs) # RA)
+      (init_rs rs: regset) m0 m1 blk sg mr
+      (CALLEESAVE: forall mr, Conventions1.is_callee_save mr ->
+                              Val.lessdef (init_rs mr.(to_preg)) (rs mr.(to_preg)))
+      (INITRSP: init_rs # RSP = Vptr blk Ptrofs.zero true)
+      (INITSIG: exists skd, skenv_link.(Genv.find_funct) (init_rs # PC) = Some skd /\ SkEnv.get_sig skd = sg)
+      (FREE: Mem.free m0 blk 0 (size_arguments sg) = Some m1)
+      (RETV: loc_result sg = One mr)
     :
-      final_frame rs_init st0 st0.(st_rs)
+      final_frame (mkstate init_rs (State rs m0)) (Retv.mk (rs mr.(to_preg)) m1)
   .
 
-  Inductive after_external (st0: state) (rs_arg: regset)
-            (rs_ret: regset) (m_ret: mem): state -> Prop :=
+  (* TODO: Push this into original compcert *)
+  Definition after_external_rs (rs0: regset): regset :=
+    fun pr =>
+      match pr.(to_mreg) with
+      | Some mr =>
+        if Conventions1.is_callee_save mr
+        then rs0 pr
+        else Vundef
+      | None =>
+        match pr with
+        | RSP => rs0 pr
+        | PC => rs0 RA
+        | _ => Vundef
+        end
+      end
+  .
+
+  Inductive after_external: state -> Retv.t -> state -> Prop :=
   | after_external_intro
+      init_rs rs0 m0 rs1 m1 retv
+      sg blk ofs
+      (SIG: exists skd, skenv_link.(Genv.find_funct) (rs0 # PC) = Some skd /\ SkEnv.get_sig skd = sg)
+      (RS: rs1 = (set_pair (loc_external_result sg) retv.(Retv.v) (after_external_rs rs0)))
+      (RSP: rs0 RSP = Vptr blk ofs true)
+      (UNFREE: Mem_unfree m0 blk ofs.(Ptrofs.unsigned) (1 + ofs.(Ptrofs.unsigned) + (size_arguments sg)) = Some m1)
     :
-      after_external st0 rs_arg rs_ret m_ret (State rs_ret m_ret)
+      after_external (mkstate init_rs (State rs0 m0))
+                     retv
+                     (mkstate init_rs (State rs1 m1))
+  .
+
+  Inductive step (ge: genv) (st0: state) (tr: trace) (st1: state): Prop :=
+  | step_intro
+      (STEP: Asm.step ge st0.(st) tr st1.(st))
+      (INITRS: st0.(init_rs) = st1.(init_rs))
   .
 
   Program Definition modsem: ModSem.t :=
     {|
-      ModSem.step := Asm.step;
-      ModSem.get_mem := get_mem;
+      ModSem.step := step;
       ModSem.at_external := at_external;
       ModSem.initial_frame := initial_frame;
       ModSem.final_frame := final_frame;
       ModSem.after_external := after_external;
-      ModSem.globalenv := ge; (* TODO: Change this properly *)
-      ModSem.skenv := (admit "TODO")
-      (* ModSem.after_external := (admit ""); *)
+      ModSem.globalenv := ge;
+      ModSem.skenv := skenv; 
     |}
   .
-  Next Obligation. all_prop_inv; ss. Qed.
-  Next Obligation. all_prop_inv; ss. Qed.
-  Next Obligation. inv FINAL0. inv FINAL1. ss. Qed.
-  Next Obligation. all_prop_inv; ss. Qed.
-  Next Obligation. ii; des; ss. inv PR; inv PR0; ss; rewrite FPTR in *; clarify. Qed.
-  Next Obligation. ii; des; ss. inv PR; inv PR0; ss; rewrite FPTR in *; clarify. Qed.
+  Next Obligation. ii; ss; des. inv_all_once; des; ss; clarify. determ_tac extcall_arguments_determ. Qed.
   Next Obligation.
-    ii; des; ss. inv PR; inv PR0; ss; rewrite FPTR in *; clarify.
-    rewrite <- RA in *. ss. des_ifs.
+    ii; ss; des. inv_all_once; des; ss; clarify.
+    rewrite INITRSP in *. clarify.
+    f_equal. rewrite RETV in *. clarify.
+  Qed.
+  Next Obligation.
+    ii; ss; des. inv_all_once; des; ss; clarify.
+    rewrite RSP in *. clarify.
+  Qed.
+  Next Obligation.
+    ii; ss; des. inv_all_once; des; ss; clarify.
+    admit "".
+  Qed.
+  Next Obligation.
+    ii; ss; des. inv_all_once; ss; clarify.
+    admit "".
+  Qed.
+  Next Obligation.
+    ii; ss; des. inv_all_once; ss; clarify.
+    admit "".
   Qed.
 
+  Lemma not_external
+    :
+      is_external ge <1= bot1
+  .
+  Proof.
+    ii. hnf in PR. des_ifs.
+    subst_locals.
+    unfold Genv.find_funct, Genv.find_funct_ptr in *. des_ifs.
+    eapply SkEnv.revive_no_external; eauto.
+  Qed.
+
+  Lemma lift_receptive_at
+        st
+        (RECEP: receptive_at (semantics_with_ge ge) st)
+    :
+      forall init_rs, receptive_at modsem (mkstate init_rs st)
+  .
+  Proof.
+    inv RECEP. i. econs; eauto; ii; ss.
+    - inv H. ss. exploit sr_receptive_at; eauto.
+      { eapply match_traces_preserved; try eassumption. ii; ss. }
+      i; des.
+      eexists (mkstate _ s2). ss.
+    - inv H. ss. exploit sr_traces_at; eauto.
+  Unshelve.
+    all: ss.
+  Qed.
+
+  Lemma modsem_receptive
+        st
+    :
+      receptive_at modsem st
+  .
+  Proof. destruct st. eapply lift_receptive_at. eapply semantics_receptive. ii. eapply not_external; eauto. Qed.
+
+  Lemma lift_determinate_at
+        st0
+        (DTM: determinate_at (semantics_with_ge ge) st0)
+    :
+      forall init_rs, determinate_at modsem (mkstate init_rs st0)
+  .
+  Proof.
+    inv DTM. i. econs; eauto; ii; ss.
+    - inv H. inv H0. ss.
+      determ_tac sd_determ_at. esplits; eauto.
+      { eapply match_traces_preserved; try eassumption. ii; ss. }
+      i. clarify. destruct s1, s2; ss. f_equal; ss. eauto.
+    - inv H. ss. exploit sd_traces_at; eauto.
+  Unshelve.
+    all: ss.
+  Qed.
+
+  Lemma modsem_determinate
+        st
+    :
+      determinate_at modsem st
+  .
+  Proof. destruct st. eapply lift_determinate_at. eapply semantics_determinate. ii. eapply not_external; eauto. Qed.
+
+
 End MODSEM.
+
+
+
+
+
+Section MODULE.
+
+  Variable p: program.
+
+  Program Definition module: Mod.t :=
+    {|
+      Mod.data := p;
+      Mod.get_sk := Sk.of_program fn_sig;
+      Mod.get_modsem := modsem;
+    |}
+  .
+  Next Obligation.
+    rewrite Sk.of_program_defs.
+    eapply SkEnv.project_impl_spec; eauto.
+  Qed.
+
+End MODULE.
+
